code/coq/attic/det.v
@@ -1,0 +1,871 @@
+From Coq Require Import FunctionalExtensionality.
+From mathcomp Require Import all_ssreflect.
+
+From det Require Import program.
+From det Require Import interpreter.
+From det Require Import aux.
+
+
+Lemma map_cat_deep {T:Type} {R:Type} l gs:
+  forall (P:T -> R),
+  [seq [seq P x | x <- b] ++ [seq P x | x <- gs] | b <- l] = [seq [seq P x | x <- b ++ gs] | b <- l].
+Proof.
+  revert gs; induction l; intros; simpl; f_equal; auto.
+  now rewrite map_cat.
+Qed.
+
+(* Definition functional_prog' p :=
+  forall n r g a, run p n g a = r -> r = None \/ r = Some a. *)
+
+Definition functional_prog p :=
+  forall n r g, run p n (not_alt_goal g) [::] = r -> r = None \/ r = Some [::].
+
+Definition functional_pred p f :=
+  forall n r, run p n [:: Goal (call f) [::]] [::] = r -> r = None \/ r = Some [::].
+
+Definition functional_goal p g :=
+  forall n r, run p n (not_alt_goal g) [::] = r -> r = None \/ r = Some [::].
+
+Definition functional_goal' p g :=
+  forall n r, run p n (not_alt_goal g) [::] = r -> r = Some [::].
+
+Lemma functional_neck_cut_all:
+  forall p, functional_prog (neck_cut_all p).
+Proof.
+  move=> prog n.
+  elim: n => /=.
+  - move=> r _ <-; auto.
+  - move=> n IH [sol|]; auto.
+    move=> [|[|p] gs] /=; auto.
+    + apply IH.
+    + simpl; unfold neck_cut_all.
+      destruct (prog p) as [|s] eqn:?; auto.
+      simpl; fold_neck_cut_all prog.
+      destruct n; auto.
+      move => /= H.
+      apply pumping1 in H.
+      specialize (IH (Some sol) (s ++ gs)).
+      rewrite <-map_cat in H.
+      now apply IH.
+Qed.
+
+Module Elpi.
+  Definition success p g a :=
+    exists x, Elpi.nur p g a x.
+
+  Definition functional_goal p g :=
+    (exists x, Elpi.nur p g [::] x) -> Elpi.nur p g [::] [::].
+
+  Lemma functional_neck_cut_all:
+    forall p g, functional_goal (neck_cut_all p) (not_alt_goal g).
+  Proof.
+    intros ??[x H].
+    remember (neck_cut_all p).
+    remember (not_alt_goal g).
+    remember [::].
+    revert g Heqb Heql0 Heql.
+    induction H.
+    - intros; subst; constructor.
+    - intros; subst; constructor.
+      destruct g; inversion Heql; subst.
+      eapply IHnur; auto.
+    - intros; subst.
+      destruct g; inversion Heql.
+      subst.
+      econstructor.
+      eapply H.
+      simpl in Heql.
+      (* econstructor 3. *)
+      (* apply H. *)
+  Abort.
+End Elpi.
+
+Definition all_pred_have_cut :=
+  for_all (exists_ (fun x => x = cut)).
+
+Definition all_rules_have_cut (p: bodiesT) :=
+  forall f, all_pred_have_cut (p f).
+
+Definition goal_has_cut :=
+  (exists_ (fun g => match g with Goal g _ => g = cut end)).
+
+Definition all_goals_have_cut l := for_all (goal_has_cut) l.
+
+Lemma all_have_cut_save_alt {b a gs} :
+  exists_ (eq^~ cut) b ->
+  goal_has_cut gs ->
+  goal_has_cut (save_alt a b gs).
+Proof.
+  unfold save_alt.
+  revert gs.
+  elim: b.
+  inversion 1.
+  move=> b bs IH gs [|CUT_B CUT_BS].
+  intros; subst.
+  constructor; auto.
+  constructor 2.
+  now apply IH.
+Qed.
+
+Lemma all_have_cut_more_alts {a bs gs} :
+  for_all (exists_ (fun x => x = cut)) (bs) -> 
+    all_goals_have_cut (gs :: a) ->
+      all_goals_have_cut (more_alt a bs gs).
+Proof.
+  unfold more_alt.
+  move=> CUT_BS [CUT_GS CUT_A].
+  induction bs as [|b bs]; auto.
+  destruct CUT_BS as [CUT_B CUT_BS].
+  constructor.
+  apply all_have_cut_save_alt; auto.
+  now apply IHbs.
+Qed.
+
+(* Lemma more_goals {prog n g gs l a1} :
+  run prog n (g++gs) a1 = Some l ->
+    (exists n' a2, n' <= n /\ run prog n' gs a2 = Some l).
+Proof.
+  revert g gs a1.
+  induction n.
+    exists 0, [::]; auto.
+  destruct g.
+    exists n.+1, a1; auto.
+  destruct g; destruct g.
+    simpl.
+    intros.
+    apply IHn in H as [?[?[]]].
+    exists x, x0; auto.
+  simpl.
+  destruct (prog n0) eqn:PP.
+    unfold more_alt, save_alt; simpl.
+    destruct a1; simpl.
+      inversion 1.
+    intros. 
+    exists (n), 
+    de
+  intros. *)
+
+Lemma succeed_hd_list {prog n s}:
+  forall hd gs a, 
+    run prog n (hd ++ gs) a = Some s ->
+      exists n', n' <= n /\
+        ((exists a', run prog n' gs a' = Some s) \/ next_alt a (run prog n') = Some s).
+Proof.
+  induction n.
+    exists 0; constructor; auto; left; exists [::]; auto.
+  destruct hd.
+    exists (n.+1); constructor; auto; left; exists a; auto.
+  destruct g as [[|p] ca].
+    (* cut case *)
+    simpl.
+    intros.
+    apply IHn in H as [?[]].
+    exists x; constructor; auto.
+Abort.
+
+Lemma succeed_hd {prog n s}:
+  forall hd gs a, 
+    run prog n (hd :: gs) a = s ->
+      exists n', n' <= n /\
+        ((exists a', run prog n' gs a' = s) \/ next_alt a (run prog n') = s).
+Proof.
+  induction n.
+    exists 0; constructor; auto; left; exists a; auto.
+  destruct hd; destruct g.
+    simpl.
+    exists n; constructor; auto; left; exists ca; auto.
+  simpl.
+  destruct (prog n0); unfold more_alt, save_alt; simpl.
+    exists n; constructor; auto; auto.
+  destruct l.
+    simpl.
+    exists n; constructor; auto; left; eexists.
+    apply H.
+  simpl.
+  intros.
+  apply IHn in H.
+  destruct H.
+  destruct H.
+  destruct H0.
+  destruct H0.
+Abort.
+
+Lemma goals_with_cut_big_step {prog n s}:
+  forall g1 g2 ca a,  
+    run prog n (g1 ++ Goal cut ca :: g2) a = s ->
+      exists n', n' <= n /\ 
+        (next_alt a (run prog n') = s \/ run prog n' g2 ca = s).
+Proof.
+  intro.
+  revert n.
+  induction g1.
+    destruct n; simpl.
+      exists 0; auto.
+    intros.
+    exists n; auto.
+  destruct n.
+    exists 0; auto.
+  destruct a; destruct g; simpl.
+    intros.
+    specialize (IHg1 _ _ _ _ H) as (?&?&?).
+    exists x.
+    constructor; auto.
+  auto.
+
+  admit.
+Abort.
+
+Lemma all_goals_with_cut_more_general' {prog g a r}:
+  all_rules_have_cut prog ->
+    all_goals_have_cut (g :: a) ->
+      Elpi.nur prog g a r ->
+      exists g', In g' (g::a) /\ Elpi.nur prog g' [::] r.
+Proof.
+  move=> ARC AGC RUN.
+  induction RUN.
+  - destruct AGC as [[] ?].
+  - exists ((Goal cut ca :: gl)); repeat constructor; auto.
+  - assert (all_goals_have_cut (gl :: a)).
+    1:{ destruct AGC as [[] ?]; try by []. }
+    clear AGC.
+    specialize (ARC f).
+    rewrite H in ARC.
+    assert (all_goals_have_cut (save_alt a b gl :: more_alt a bs gl)).
+      apply (@all_have_cut_more_alts) with (bs:=b :: bs); auto.
+    specialize (IHRUN H1) as (?&?&?).
+    exists x.
+    constructor; auto.
+    revert H2.
+    unfold more_alt, save_alt.
+
+    admit.
+  - destruct AGC as [AGC1 AGC2].
+    destruct (IHRUN AGC2) as [?[]].
+    exists x.
+    constructor; auto.
+    simpl.
+    auto.
+Abort.
+
+Inductive IN_IND (prog: bodiesT) : list goal -> ( seq (seq goal)) -> Prop :=
+  | IN_IND_OK g gs: IN_IND g (g::gs)
+  | IN_IND_KO g ign gs: IN_IND g gs -> IN_IND g (ign::gs)
+  | IN_IND_RC ca (a:seq (seq goal)) p g gs tl :
+      IN_IND g ([seq [seq Goal x a | x <- x] ++ tl | x <- prog p] ++ gs) ->
+        IN_IND g ((Goal (call p) ca :: tl) :: gs)
+  .
+
+
+Lemma all_goals_with_cut_more_general' {prog g a r}:
+  all_rules_have_cut prog ->
+    all_goals_have_cut (g :: a) ->
+      Elpi.nur prog g a r ->
+      exists g', IN_IND prog g' (g::a) /\ Elpi.nur prog g' [::] r.
+Proof.
+  move=> ARC AGC RUN.
+  induction RUN.
+  - destruct AGC as [[] ?].
+  - exists ((Goal cut ca :: gl)); repeat constructor; auto.
+  - assert (all_goals_have_cut (gl :: a)).
+    1:{ destruct AGC as [[] ?]; try by []. }
+    clear AGC.
+    specialize (ARC f).
+    rewrite H in ARC.
+    assert (all_goals_have_cut (save_alt a b gl :: more_alt a bs gl)).
+      apply (@all_have_cut_more_alts) with (bs:=b :: bs); auto.
+    specialize (IHRUN H1) as (?&?&?).
+    exists x.
+    constructor; auto.
+    revert H2.
+    unfold more_alt, save_alt.
+    intro.
+    econstructor 3.
+    rewrite H.
+    apply H2.
+  - destruct AGC as [AGC1 AGC2].
+    destruct (IHRUN AGC2) as [?[]].
+    exists x.
+    constructor; auto.
+    constructor; auto.
+Abort.
+
+Lemma all_goals_with_cut_more_general'' {prog n g a r}:
+  all_rules_have_cut prog ->
+    all_goals_have_cut (g :: a) ->
+      run prog n g a = r ->
+      exists g' n', IN_IND prog g' (g::a) /\ run prog n' g' [::] = r. (*TODO: add: n' <= n*)
+Proof.
+  revert g a r.
+  induction n.
+  + intros; simpl in H1; subst; exists g, 0; repeat constructor.
+  + simpl.
+    destruct g.
+    intros; destruct H0 as [[]?].
+  + destruct g; destruct g.
+    * intros.
+      exists ((Goal cut ca :: g0)), (n.+1); repeat constructor; auto.
+    * intros.
+      destruct (prog n0) eqn:PP.
+        unfold more_alt in H1; simpl in H1.
+        destruct a; simpl in *.
+          exists (Goal (call n0) ca::g0), 0; split; auto; repeat constructor.
+        destruct H0.
+        epose proof (IHn _ _ _ H H2 H1).
+        destruct H3 as (?&?&?&?).
+        exists x,x0; constructor; auto.
+        econstructor 3; auto.
+        rewrite PP; auto.
+      --- (*non empty prog*)
+      simpl in H1.
+      epose proof (IHn _ _ _ H _ H1) as (?&?&?&?).
+      exists x,x0; constructor; auto.
+      econstructor 3.
+      rewrite PP.
+      apply H2.
+      Unshelve.
+      2:{
+          epose proof (@all_have_cut_more_alts a (l::l0) g0) as HH.
+          eapply HH.
+          specialize (H n0); rewrite PP in H; auto.
+          inversion H0.
+          inversion H2.
+          inversion H4.
+          constructor; auto.
+        }
+        apply [::].
+Qed.
+
+(* in all goal (g::gs) we have a bang and each of them has no cut-alternatives,
+      therefore, 
+        -if a goal g' in (g::gs) succeeds, we have
+          the same result as running the goal g' alone (the alternative being rejected)
+        -otherwise, if all goals fails, the lemma is trivial
+      
+  *)
+Lemma all_goals_with_cut prog n r:
+  forall g gs tl, all_rules_have_cut prog ->
+    all_pred_have_cut (g :: gs) ->
+      run prog n (not_alt_goal (g ++ tl))
+        (more_alt [::] gs (not_alt_goal tl)) = r ->
+        (* [seq [seq Goal x [::]  | x <- b] ++ not_alt_goal tl | b <- gs] = r -> *)
+        exists g n', n' <= n /\ run prog n' (not_alt_goal g) [::] = r.
+Proof.
+  induction n.
+    now exists [::], 0; auto.
+  destruct g; simpl.
+    now destruct 2 as [[] ?].
+  destruct p as [|p]; simpl.
+    now intros; exists (cut :: g ++ tl), (n.+1); auto.
+  destruct (prog p) eqn:PP.
+    destruct 2 as [[] ?]; try by [].
+    unfold more_alt; simpl.
+    destruct gs; simpl.
+      now exists [::], 0; auto.
+    unfold save_alt.
+    rewrite <-map_cat.
+    intro.
+    epose proof (IHn _ _ _ H H1 H2).
+    destruct H3 as (gg&nn&?&?).
+    now exists gg,nn; auto.
+  simpl.
+  destruct 2 as [[]?]; [by[]|].
+  epose proof (IHn _ _ _ H (conj H0 H1)).
+  intros.
+  
+
+Admitted.
+
+Section CUT_PROG.
+
+  Context {prog : bodiesT}.
+  Context (CProg : all_rules_have_cut prog).
+
+  Lemma goals_with_cut_big_step {n s}:
+    forall g1 g2 ca,  
+      run prog n ([seq Goal g ca | g <- g1] ++ Goal cut ca :: g2) ca = Some s ->
+        exists n', n' <= n /\ 
+          (next_alt ca (run prog n') = Some s \/ run prog n' g2 ca = Some s).
+  Proof.
+    induction n.
+      exists 0; auto.
+    destruct g1 as [|hd g1]; simpl.
+      exists n; auto.
+    (* g1 is not empty: hd::g1 *)
+    destruct hd.
+      (* hd is a cut *)
+      intros.
+      apply IHn in H as [?[?[]]].
+      exists x; auto.
+      exists x; auto.
+    (*hd is call*)
+    destruct (prog n0) eqn:PP.
+      unfold more_alt; simpl.
+      exists n; auto.
+    simpl.
+    unfold save_alt; simpl.
+    (* Search ((_++_)++_). *)
+    intros.
+    rewrite catA in H.
+  Abort.
+
+  Lemma starts_with_cut {n s}:
+    forall g2 ca a,  
+      run prog n (Goal cut ca :: g2) a = Some s ->
+        exists n', n' <= n /\ 
+          (run prog n' g2 ca = Some s).
+  Proof.
+    induction n.
+      by[].
+    now exists n; auto.
+  Qed.
+
+  Lemma starts_with_call {n s}:
+    forall p g2 ca a,
+      run prog n (Goal (call p) ca :: g2) a = Some s ->
+        exists n', n' <= n /\ 
+          (next_alt (more_alt a (prog p) g2) (run prog n') = Some s).
+  Proof.
+    induction n.
+      now by [].
+    exists n; auto.
+  Qed.
+
+  (* Lemma add_cut_change_nothing:
+    run prog n2 cut (alt1 ++ aft) = Some alt2 ->
+      exists n3 : nat, run prog n3 [::] (alt1 ++ cut :: aft) = Some alt2. *)
+
+
+  Inductive split_cut : list alt -> list alt -> alt -> list alt -> Prop :=
+    | split_cut_lst hd tl : goal_has_cut hd -> split_cut (hd::tl) [::] hd tl
+    | split_cut_not hd tl : forall bef cut aft,
+      not (goal_has_cut hd) -> split_cut tl bef cut aft ->
+        split_cut (hd::tl) (hd::bef) cut aft.
+
+  Lemma split_cut_app:
+    forall l bef cut aft,
+      split_cut l bef cut aft -> (l = bef ++ cut :: aft).
+  Proof.
+    (* constructor. *)
+    induction 1; intros; auto; simpl; f_equal; auto.
+  Qed.
+
+  Lemma fail_or_succeed {n1 n2}:
+    forall l bef cut aft alt1 alt2,
+      split_cut l bef cut aft ->
+        next_alt bef (run prog n1) = Some alt1 ->
+          next_alt (more_alt (alt1++cut::aft) [::] [::]) (run prog n2) = Some alt2 ->
+            exists n3, next_alt (more_alt l [::] [::]) (run prog n3) = Some alt2.
+  Proof.
+    revert n2.
+    induction n1 as [|n1]; destruct bef as [|bef befs]; try by [].
+    destruct bef as [|b bs]; simpl.
+      (*bef = [::]; befs = any; alt1 = befs *)
+      intros cut aft alt1 alt2 HSplit.
+      inversion HSplit.
+      apply split_cut_app in HSplit as HSplitCat; subst.
+      inversion HSplitCat; subst; clear HSplitCat.
+      inversion 1.
+      simpl.
+      exists 4; simpl.
+  Abort.
+
+  Lemma fail_or_succeed {n1 n2 s} r:
+    forall g1 g2 ca,
+      (for_all (fun x => match x with Goal g _ => g <> cut end) g1) ->
+      run prog n1 g1 ca = Some (s ++ ca) ->
+          run prog n2 g2 (s ++ ca) = r ->
+            exists n3, 
+              run prog n3 (g1 ++ g2) ca = r.
+  Proof.
+    revert s n2.
+    induction n1.
+      inversion 2.
+    destruct g1; simpl.
+      destruct s; simpl; inversion 2.
+      exists n2; auto.
+      admit.
+    destruct 1 as [DIFF_CUT_HD DIFF_CUT_TL].
+    destruct g as [[]?].
+      by [].
+    destruct (prog n) eqn:PP.
+      unfold more_alt, save_alt; simpl.
+      destruct ca.
+        inversion 1.
+      simpl.
+      rewrite <-cat_rcons.
+      intros.
+      epose proof (IHn1 _ _ _ _ _ _ H H0).
+      intros.
+      inversion H0.
+      admit.
+    simpl.
+      intros.
+  Abort.
+
+  (* Lemma starts_with_call {n s}:
+    forall p g2 ca a hd tl,
+      run prog n (Goal (call p) ca :: g2) a = Some s ->
+        prog p = (hd::tl) ->
+          exists n', n' <= n /\ 
+            (next_alt (more_alt a (prog p) gs) (run prog n)).
+  Proof.
+    induction n.
+      inversion 1.
+    simpl.
+    exists n; auto.
+    rewrite H0 in H.
+    unfold more_alt in H.
+    simpl in H.
+    auto.
+  Abort. *)
+
+  Lemma with_cut l:
+    exists_ (eq^~ cut) l -> exists bef aft, (for_all (fun x => x <> cut) bef) /\ bef ++ cut :: aft = l.
+  Proof.
+    induction l; inversion 1; subst.
+      exists [::], l; simpl; auto.
+    apply IHl in H0 as [?[?[]]]; subst.
+    destruct a.
+    exists [::], (x++cut::x0); constructor; simpl; auto.
+    exists (call n::x), x0; simpl; repeat constructor; auto.
+    easy.
+  Qed.
+
+  Lemma succeed_or_fail {n1 bef aft l0 gs l1}:
+    all_pred_have_cut ((bef ++ cut :: aft) :: l0) ->
+      for_all (fun x : pred => x <> cut) bef ->
+        run prog n1 (save_alt [::] (bef ++ cut :: aft) (not_alt_goal gs))
+          [seq save_alt [::] b (not_alt_goal gs)  | b <- l0] = Some l1 ->
+        exists n2, 
+          (run prog n2 (save_alt [::] (bef ++ cut :: aft) (not_alt_goal gs)) [::] = Some l1)
+            \/
+          (next_alt [seq save_alt [::] b (not_alt_goal gs)  | b <- l0] (run prog n2) = Some l1).
+  Proof.
+    revert bef aft l0 gs l1.
+    induction n1.
+      by [].
+    simpl.
+    destruct bef; simpl.
+      exists n1.+1; auto.
+    destruct p.
+      inversion 2; by [].
+    unfold more_alt, save_alt; simpl.
+    destruct (prog n); simpl.
+      admit.
+    destruct l; simpl.
+  Admitted.
+
+  Lemma xx {l0 l1 x gs}:
+    for_all (exists_ (eq^~ cut)) l0 ->
+      next_alt [seq save_alt [::] b gs  | b <- l0] (run prog x) = Some l1 -> 
+        exists n0 g, run prog n0 (not_alt_goal g) [::] = Some l1.
+  Proof.
+    revert l0 l1 gs.
+    induction x; destruct l0 as [|hd tl]; try by [].
+    destruct hd as [|hd1 hds].
+      now inversion 1.
+    destruct hd1 as [|p].
+      (* simpl.
+      intros.
+      destruct H.
+      epose proof (IHx (hds::tl) _ gs _ _) as [?[]].
+      exists x0,x1; apply H2.
+      Unshelve.
+      3:{
+        simpl.
+        unfold save_alt.
+        admit.
+      }
+      2:{
+        
+      } *)
+        admit.
+    simpl.
+    destruct 1 as [[]?].
+      by [].
+    destruct (prog p) eqn:PP.
+      unfold more_alt, save_alt; simpl.
+      intros.
+      eapply (IHx _ _ _ H0) in H1 as [?[]].
+      exists x0, x1; auto.
+    simpl.
+    (* pose [seq save_alt [::] b (not_alt_goal gs)  | b <- tl] as T.
+    fold T.
+    pose ([seq Goal x0 [::]  | x0 <- hds] ++ not_alt_goal gs) as R.
+    fold R.
+    pose proof (CProg p).
+    rewrite PP in H1.
+    inversion H1.
+    destruct l.
+      by [].
+    unfold save_alt; simpl.
+    epose proof (IHx ((p0 :: l) :: l0) _ ) as TTT; simpl in TTT.
+    unfold save_alt in TTT.
+    simpl in TTT.
+
+    fold T R in TTT. *)
+Admitted.
+
+  Lemma bah1 {n l l0 gs l1}:
+    all_pred_have_cut (l :: l0) ->
+      run prog n (save_alt [::] l (not_alt_goal gs))
+        [seq save_alt [::] b (not_alt_goal gs)  | b <- l0] = Some l1 ->
+          exists g n, run prog n (not_alt_goal g) [::] = Some l1.
+  Proof.
+    intro.
+    inversion H.
+    apply with_cut in H0 as [bef[aft [N_CUT <-]]].
+    intros.
+    epose proof (succeed_or_fail H N_CUT H0) as [?[]].
+      unfold save_alt in H2.
+      rewrite <-map_cat in H2.
+      exists ((bef ++ cut :: aft) ++ gs), x; auto.
+
+    eapply xx in H2.
+    destruct H2 as [?[]].
+    exists x1, x0; auto.
+    auto.
+  Abort.
+
+  Inductive valid_tl : seq (seq pred) -> seq alt -> Prop :=
+    | valid_tl_base ff gs l0 : valid_tl [::] [seq save_alt ff b [seq Goal x ff  | x <- gs]  | b <- l0]
+    | valid_tl_recu l0 l2 R bef: 
+          valid_tl bef l2 -> 
+            valid_tl l0 ([seq save_alt l2 b R | b <- l0] ++ l2).
+
+  Lemma bah12 {n T R LOC_HD LOC_TL res A}:
+    all_pred_have_cut (LOC_HD :: LOC_TL) ->
+      valid_tl LOC_TL A ->
+        run prog n (save_alt T LOC_HD R) A = Some res ->
+        (* run prog n (save_alt ff l [seq Goal x ff | x <- gs])
+          [seq save_alt ff b [seq Goal x ff | x <- gs]  | b <- l0] = Some res -> *)
+            exists g n', n' <= n /\ run prog n' (save_alt T g R) T = Some res.
+  Proof.
+    revert LOC_HD LOC_TL T R res A.
+    induction n.
+      by [].
+    simpl.
+    unfold save_alt.
+    destruct LOC_HD as [|LOC_HD l0s]; simpl.
+      destruct R; now inversion 1.
+    destruct LOC_HD as [|p].
+      intros.
+      exists l0s, n; auto.
+    destruct (prog p) eqn:PP.
+      unfold more_alt; simpl.
+      destruct A as [|a A]; simpl.
+        by [].
+      inversion 2; subst.
+  Abort.
+
+  Inductive help : _ -> _ -> Prop :=
+    (* | base A G GS : help ([::]) (more_alt A G GS) *)
+    | hhhh A G GS G0 G0s PP:
+      help (more_alt A G GS) (more_alt ([seq [seq Goal x A  | x <- b] ++ GS  | b <- G0s] ++ A) PP
+([seq Goal x A  | x <- G0] ++ GS))
+    (* | recu GS G AA BB l0 L' a b : 
+      (* help a b -> *)
+      help (([seq save_alt GS b [seq Goal x a | x <- G] | b <- ((AA::BB)::l0)] ++ GS))
+        (([seq save_alt ([seq save_alt GS b G | b <- l0] ++ GS) b1 ([seq Goal x GS | x <- BB] ++ G) | b1 <- L']
+      ++ [seq save_alt GS b G | b <- l0] ++ GS)). *)
+      .
+
+  Lemma invariant_next_alt {n l1 A G GS}:
+    (* all_pred_have_cut (alts) ->
+      all_goals_have_cut ff -> *)
+        next_alt (more_alt A G GS) (run prog n) = Some l1 ->
+          False.
+  Proof.
+    remember (more_alt A G GS).
+    (* l = [seq save_alt A b GS  | b <- G] ++ A *)
+    destruct G as [|G0 G0s] eqn:LL; simpl.
+      admit.
+    rewrite Heql.
+    unfold more_alt.
+    destruct n; simpl.
+      by [].
+    destruct G0; unfold save_alt; simpl.
+      admit.
+    destruct p; [admit|].
+    unfold more_alt.
+    destruct (prog n0); [admit|].
+
+    assert (exists x, help (x) (([seq save_alt ([seq [seq Goal x A  | x <- b0] ++ GS  | b0 <- G0s] ++ A) b
+([seq Goal x A  | x <- G0] ++ GS)
+ | b <- l0 :: l2] ++ [seq [seq Goal x A  | x <- b] ++ GS  | b <- G0s] ++ A))).
+    eexists; constructor.
+    clear H.
+
+    (* next_alt (save_alt GS l G :: ([seq save_alt GS b G | b <- l0] ++ GS)) (run prog n) = Some l1 -> False *)
+    simpl map.
+    simpl.
+    destruct l0 as [|AA BB]; [admit|].
+    unfold save_alt at 1; simpl.
+    destruct n; simpl.
+      by[].
+    destruct AA; [admit|].
+
+    assert (exists x, help x (more_alt
+([seq save_alt ([seq [seq Goal x A  | x <- b0] ++ GS  | b0 <- G0s] ++ A) b
+([seq Goal x A  | x <- G0] ++ GS)
+ | b <- l2] ++ [seq [seq Goal x A  | x <- b] ++ GS  | b <- G0s] ++ A) (prog n1)
+([seq Goal x ([seq [seq Goal x0 A  | x0 <- b] ++ GS  | b <- G0s] ++ A)  | x <- BB] ++
+[seq Goal x A  | x <- G0] ++ GS))).
+
+    eexists.
+    constructor.
+    Abort.
+
+  (* Lemma bah12 {n T R LOC_HD LOC_TL res A}:
+    all_pred_have_cut (LOC_HD :: LOC_TL) ->
+      valid_tl LOC_TL A ->
+        run prog n (save_alt T LOC_HD R) A = Some res ->
+        (* run prog n (save_alt ff l [seq Goal x ff | x <- gs])
+          [seq save_alt ff b [seq Goal x ff | x <- gs]  | b <- l0] = Some res -> *)
+            exists g n', n' <= n /\ run prog n' (save_alt T g R) T = Some res.
+  Proof.
+    revert LOC_HD LOC_TL T R res A.
+    induction n.
+      by [].
+    simpl.
+    unfold save_alt.
+    destruct LOC_HD as [|LOC_HD l0s]; simpl.
+      destruct R; now inversion 1.
+    destruct LOC_HD as [|p].
+      intros.
+      exists l0s, n; auto.
+    destruct (prog p) eqn:PP.
+      unfold more_alt; simpl.
+      destruct A as [|a A]; simpl.
+        by [].
+      inversion 2; subst.
+  Admitted. *)
+
+
+  Lemma bah1 {n g alts gs l1 ff}:
+    all_pred_have_cut (g :: alts) ->
+      all_goals_have_cut ff ->
+      run prog n (save_alt ff g [seq Goal x ff | x <- gs])
+        [seq save_alt ff b [seq Goal x ff | x <- gs]  | b <- alts] = Some l1 ->
+          exists g n', n' <= n /\ run prog n' [seq Goal x ff | x <- g] ff = Some l1.
+  Proof.
+    (* intros.
+    epose proof (bah12 _ _ H1) as [?[?[]]].
+    unfold save_alt in H3.
+    rewrite <-map_cat in H3.
+    exists (x++gs), x0; auto.
+    Unshelve.
+    3:{ constructor. }
+    inversion H; auto.
+    constructor; auto.
+    constructor. *)
+
+    revert g alts gs l1 ff.
+    induction n.
+      by [].
+    simpl.
+    unfold save_alt.
+    destruct g.
+      now inversion 1.
+    simpl.
+    destruct p.
+      intros.
+      exists (g++gs), n. rewrite <-map_cat in H1; auto.
+    destruct (prog n0) eqn:PP.
+      unfold more_alt; simpl.
+      destruct alts.
+        by [].
+      simpl.
+      inversion 1.
+      intros.
+      eapply IHn in H3 as [?[?[]]].
+      exists x, x0; auto.
+      all:auto.
+    simpl.
+    intros.
+    rewrite <-map_cat in H1.
+    rewrite map_cat_deep in H1.
+    pose ([seq [seq Goal x ff  | x <- b ++ gs] | b <- alts]) as T; fold T in H1.
+    pose ([seq Goal x ff  | x <- g++gs]) as R; fold R in H1.
+    
+    (* Se solo riuscissi a risolvere questo... *)
+
+  Admitted.
+
+  Lemma bah {n l l0 gs l1}:
+    all_pred_have_cut (l :: l0) ->
+      run prog n (save_alt [::] l (not_alt_goal gs))
+        [seq save_alt [::] b (not_alt_goal gs)  | b <- l0] = Some l1 ->
+          exists g, run prog n (not_alt_goal g) [::] = Some l1.
+  Proof.
+    (* intros.
+    assert (all_goals_have_cut [::]).
+    constructor.
+    epose proof (bah1 H H1 H0) as (?&?&?&?).
+    apply (pumping_leq _ _ _ _ _ _ H2) in H3.
+    exists x; auto. *)
+    revert l l0 gs l1.
+    induction n; try by [].
+    destruct l; unfold save_alt; simpl.
+      inversion 1; by [].
+    destruct p; intros l0 gs l1; rewrite <-map_cat.
+      exists (cut :: l ++ gs); simpl; auto.
+    destruct (prog n0) eqn:PP; simpl.
+      unfold more_alt.
+      destruct l; inversion 1.
+        inversion H0; by [].
+      destruct l0; try by [].
+      simpl.
+      unfold save_alt in IHn.
+      intro.
+      eapply IHn in H2 as []; auto.
+      (* if the goal is (p, !) and p fails then go to the choice point *)
+      exists (cut :: x); simpl; auto.
+      repeat rewrite map_cat_deep.
+      pose ([seq [seq Goal x [::]  | x <- b ++ gs]  | b <- l0]) as T1; fold T1.
+      pose ([seq Goal x [::]  | x <- l ++ gs]) as T2; fold T2.
+
+      (*qui è difficile...*)
+  Admitted.
+
+  Lemma functional_all_with_cut: functional_prog prog.
+  Proof.
+    intros n.
+    induction n; auto.
+    destruct g as [|g gs]; simpl; auto.
+    destruct g as [|p].
+      apply IHn.
+    destruct (prog p) eqn:?; auto.
+    simpl; rewrite cats0.
+    destruct r; auto.
+    pose proof (CProg p) as Hp.
+    rewrite Heql in Hp.
+    intro.
+    epose proof (bah Hp H) as [g HP].
+    apply IHn in HP; auto.
+  Qed.
+End CUT_PROG.
+
+Lemma all_have_cut_tail_cut_all:
+  forall p, all_rules_have_cut(tail_cut_all p).
+Proof.
+  intros ??.
+  unfold tail_cut_all.
+  destruct (p f); simpl; auto.
+  split.
+  constructor.
+  induction l; simpl; auto.
+
+  induction l0; simpl; auto.
+  constructor; auto.
+  induction a; simpl; auto.
+Qed.
+
+Lemma functional_tail_cut_all:
+  forall p, functional_prog (tail_cut_all p).
+Proof.
+  intro.
+  
+  eapply (functional_all_with_cut).
+  apply all_have_cut_tail_cut_all.
+Qed.
